\documentclass{article}

\usepackage[fleqn]{amsmath}
\usepackage{syn}

\usepackage{enumerate}

% only one of the two following two lines is necessary; txfonts has better glyphs
% \usepackage{stmaryrd}
\usepackage{txfonts}

\usepackage{fullpage}
\usepackage{proof}

\setlength{\parindent}{0pt}
\setlength{\parskip}{6pt}

\allowdisplaybreaks[4]

\title{proof rewriting -- $\mathbf 1$-normal form}
\author{Kaustuv Chaudhuri}

\begin{document}

\maketitle

\sdef{G}{\Gamma}
\sdef{D}{\Delta}
\sdef{|-}{\vdash}

\sdef{==>}{\Longrightarrow}
\sdef{<==}{\Longleftarrow}

\sdef{aa}{\alpha}
\sdef{bb}{\beta}
\sdef{cc}{\gamma}

\sdef{/}{\mathbin{\backslash}}
\sdef{;}{\mathbin{\mathbf{;}}}
\sdef{and}{\wedge}
\sdef{or}{\vee}

\makeatletter
\let\I@align=\vbox
\def\Ic{\let\I@align=\vcenter\I}
\newcommand{\I}[2][]{\def\I@args{[#1]{#2\mathstrut}}\I@more}
\def\I@more{\@ifnextchar\bgroup\I@pre\I@nopre}
\def\I@nopre{\expandafter\I@\I@args{}}
\def\I@pre#1{\expandafter\I@\I@args{#1\mathstrut}}
\def\I@[#1]#2#3{\I@align{\let\I@align=\vbox\infer[#1]{#2}{#3}}}
\makeatother

\sdef{tens}{\otimes}

\sdef{one}{\mathbf{1}}
\sdef{zero}{\mathbf{0}}

\sdef{top}{\top}

\sdef{-o}{\multimap}
\sdef{with}{\mathbin{\&}}
\sdef{fst}{\mathop{\mathbf{fst}}}
\sdef{snd}{\mathop{\mathbf{snd}}}

\sdef{let}{\mathbf{let}\,}
\sdef{in}{\mathbin{\mathbf{in}}}
\sdef{end}{\,\mathbin{\mathbf{end}}}

\sdef{choice}{\oplus}
\sdef{inl}{\mathop{\mathbf{inl}}}
\sdef{inr}{\mathop{\mathbf{inr}}}
\sdef{case}{\mathbf{case}\,}
\sdef{of}{\mathbin{\mathbf{of}}}
\sdef{=>}{\mathbin{\Rightarrow}}
\sdef{|}{\mathbin{|}}

\sdef{abort}{\mathop{\mathbf{abort}}}

\sdef{lam}#1.{\lambdaup #1.\;}

\sdef{fn}#1.{\mathtt{fn}\;#1 \Rightarrow  }

\def\SP{\hspace{2em plus 1em minus 1.5em}}

\sdef{bar}#1{\overline{#1}}
\sdef{onf}#1{\mathop{\mathsf{onf}}{(#1)}}
\def\<{\left[}
\def\>{\right]}

\sdef{ml}#1{\mathtt{#1}}
\sdef{->}{\rightarrow}

"onf A = \< bar A, f, g \>" such that "f ==> A -o bar A" and "g ==> bar A -o A"

\begin{enumerate}[{\underline{\textit{Case}}}.\ ]
\item "A = P" or a constant; i.e., "bar A = A":
  \begin{gather*}
    "onf A = \< A, ( lam u. u : A -o A ), ( lam u. u : A -o A ) \>"
  \end{gather*}


\item "A = B tens C".
  \begin{align*}
    "onf B" &= "\< bar B, f_B, g_B \>" \\
    "onf C" &= "\< bar C, f_C, g_C \>"
  \end{align*}
  \begin{enumerate}[{\underline{\textit{Subcase}}}.\ ]
  \item "bar B = one", i.e., "bar{B tens C} = bar C":
    \begin{gather*}
      "onf A" =
      \< \begin{array}{l}
           "bar C", \\
           "\left( lam u. let v_1 tens v_2 = u in let one = f_B\ v_1 in f_C\ v_2 end end : B tens C -o bar C \right)",\\
           "\left( lam u. g_B\ one tens g_C\ u : bar C -o B tens C \right)"
         \end{array} \>
    \end{gather*}

  \item "bar C = one", i.e., "bar{B tens C} = bar B":
    \begin{gather*}
      "onf R" =
      \< \begin{array}{l}
           "bar B", \\
           "\left( lam u. let v_1 tens v_2 = u in let one = f_C\ v_2 in f_B\ v_1 end end : B tens C -o bar B \right)",\\
           "\left( lam u. g_B\ u tens g_C\ one : bar B -o B tens C \right)"
         \end{array} \>
    \end{gather*}

  \item neither "bar B = one" nor "bar C = one", i.e., "bar{B tens C} = bar B tens bar C":
    \begin{gather*}
      "onf A" =
      \< \begin{array}{l}
           "bar B tens bar C", \\
           "\left( lam u. let v_1 tens v_2 = u in f_B\ v_1 tens f_C\ v_2 end : B tens C -o bar B tens bar C \right)",\\
           "\left( lam u. let v_1 tens v_2 = u in g_B\ v_1 tens g_C\ v_2 end : bar B tens bar C -o B tens C \right)"
         \end{array} \>
    \end{gather*}
  \end{enumerate}


\item "A = B -o C".
  \begin{align*}
    "onf B" &= "\< bar B, f_B, g_B \>" \\
    "onf C" &= "\< bar C, f_C, g_C \>"
  \end{align*}

  \begin{enumerate}[{\underline{\textit{Subcase}}}.\ ]
  \item "bar B = one", i.e., "bar{B -o C} = bar C":
    \begin{gather*}
      "onf A" =
      \< \begin{array}{l}
           "bar C", \\
           "\left( lam u. f_C\ ( u\ ( g_B\ one ) ) : (B -o C) -o bar C \right)",\\
           "\left( lam u. lam v. let one = f_B\ v in g_C\ u end : bar C -o B -o C \right)"
         \end{array} \>
    \end{gather*}

  \item "bar B \neq one", i.e., "bar{B -o C} = bar B -o bar C":
    \begin{gather*}
      "onf A" =
      \< \begin{array}{l}
           "bar B -o bar C", \\
           "\left( lam u. lam v. f_C\ ( u\ ( g_B\ v ) ) : (B -o C) -o bar B -o bar C \right)",\\
           "\left( lam u. lam v. g_C\ ( u\ ( f_B\ v ) ) : ( bar B -o bar C) -o B -o C \right)"
         \end{array} \>
    \end{gather*}
  \end{enumerate}

\item "A = B with C".
  \begin{align*}
    "onf B" &= "\< bar B, f_B, g_B \>" \\
    "onf C" &= "\< bar C, f_C, g_C \>"
  \end{align*}

  \begin{enumerate}[{\underline{\textit{Subcase}}}.\ ]
  \item "bar B = bar C = one", i.e., "bar{B with C} = one":
    \begin{gather*}
      "onf A" =
      \< \begin{array}{l}
           "one", \\
           "\left( lam u. f_B\ ( fst u ) : B with C -o one \right)",\\
           "\left( lam u. ( g_B\ u, g_C\ one ) : one -o B with C \right)"
         \end{array} \>
    \end{gather*}

  \item either "bar B \ne one" or "bar C \ne one", i.e., "bar{B with C} = bar B with bar C":
    \begin{gather*}
      "onf A" =
      \< \begin{array}{l}
           "bar B with bar C", \\
           "\left( lam u. ( f_B\ ( fst u ), f_C\ ( snd u ) ) : B with C -o bar B with bar C \right)",\\
           "\left( lam u. ( g_B\ ( fst u ), g_C\ ( snd u ) ) : bar B with bar C -o B with C \right)"
         \end{array} \>
    \end{gather*}
  \end{enumerate}

\item "A = B choice C".
  \begin{align*}
    "onf B" &= "\< bar B, f_B, g_B \>" \\
    "onf C" &= "\< bar C, f_C, g_C \>"
  \end{align*}

  \begin{enumerate}[{\underline{\textit{Subcase}}}.\ ]
  \item "bar B = bar C = one", i.e., "bar{B choice C} = one":
    \begin{gather*}
      "onf A" =
      \< \begin{array}{l}
           "one", \\
           "\left( lam u. case u of inl v_1 => f_B\ v_1 | inr v_2 => f_C\ v_2 : B choice C -o one \right)",\\
           "\left( lam u. inl ( g_B\ one ) : one -o B choice C \right)"
         \end{array} \>
    \end{gather*}

  \item either "bar B \ne one" or "bar C \ne one", i.e., "bar{B choice C} = bar B choice bar C":
    \begin{gather*}
      "onf A" =
      \< \begin{array}{l}
           "bar B choice bar C", \\
           "\left( lam u. case u of inl v_1 => inl ( f_B\ v_1 ) | inr v_2 => inr ( f_C\ v_2 )
                   : B choice C -o bar B choice bar C \right)",\\
           "\left( lam u. case u of inl v_1 => inl ( g_B\ v_1 ) | inr v_2 => inr ( g_C\ v_2 )
                   : bar B choice bar C -o B choice C \right)"
         \end{array} \>
    \end{gather*}
  \end{enumerate}

\item "A = {!B}".
  \begin{gather*}
    "onf B = \< bar B, f_B, g_B \>"
  \end{gather*}

  \begin{enumerate}[{\underline{\textit{Subcase}}}.\ ]
  \item "bar B = one", i.e., "bar{!B} = one":
    \begin{gather*}
      "onf A" = 
      \< \begin{array}{l}
           "one", \\
           "\left( lam u. let !v = u in f_B\ v end : {!B} -o one \right)",\\
           "\left( lam u. let one = u in {! ( g_B one )} end : one -o {!B} \right)"
         \end{array} \>
    \end{gather*}

  \item "bar B \neq one", i.e., "bar{!B} = {! bar B}":
    \begin{gather*}
      "onf A" = 
      \< \begin{array}{l}
           "one", \\
           "\left( lam u. let !v = u in {! ( f_B\ v )} end : {!B} -o {! bar B} \right)",\\
           "\left( lam u. let !v = u in {! ( g_B\ v )} end : {! bar B} -o {!B} \right)"
         \end{array} \>
    \end{gather*}
  \end{enumerate}
\end{enumerate}


\end{document}
